\documentclass{article}

\usepackage[letterpaper, margin=1.3cm]{geometry}
\usepackage[utf8]{inputenc}
\usepackage{siunitx}
\usepackage{mathtools}
\usepackage{multicol}

\title{ECE 240 Assignment 8}
\author{Michael Kwok}
\begin{document}

\maketitle
\begin{multicols}{2}
\section*{1}
\begin{align*}
F(s) &= \int_{0^-}^\infty f(t)e^{-st}dt\\
&= \int_{0^-}^\infty \left(e^{2t} -2e^{-t}\right)e^{-st} u(t)dt\\
&= \int_{0}^\infty e^{-(s-2)t}dt - 2\int_{0}^\infty e^{-(1+s)t}dt\\
&= \left[\frac{1}{s-2}e^{-(s-2)t}\right]^\infty_0 + \left[ \frac{1}{1+s}e^{-(s+1)t}\right]^\infty_0
\end{align*}

The first expression is only convergent when $s-2 > 0$. Since $s = \sigma + j\omega$, the region of convergence will be calculated by the following:
 
\begin{align*}
    \sigma -2 &> 0\\
    \sigma &> 2
\end{align*}

So assuming $\sigma > 2$,

\begin{align*}
    F(s) &= \frac{1}{s-2} \lim_{t \to \infty} \left( e^{-(s-2)t} -1 \right)\\
    &+ \frac{2}{s+1} \lim_{t \to \infty} \left( e^{-(s+1)t} -1 \right)\\
    &= \boxed{\frac{1}{s-2} - \frac{2}{s+1}}
\end{align*}
\section*{2}
\begin{align*}
    f(t) &= \int_0^1 te^{-t}dt + \int_1^\infty e^{-t}dt\\
    &= e^{-1}\left(\frac{1}{2} - 0\right) + \lim_{t\to\infty}\left(-e^{-t} + e^{-1}\right)\\
    &= \frac{1}{2} e^{-1} + e^{-1}\\
    &= \boxed{\frac{3}{2}e^{-1}}
\end{align*}
\section*{3}
\subsection*{a}
\begin{align*}
    f_1(t) &= \sin\left[\omega_0(t-\tau)\right]u(t-\tau)\\
    F_1(s) &= \boxed{\frac{\omega_0}{s^2 + \omega_0^2} e^{-s\tau}}
\end{align*}
\subsection*{b}
\begin{align*}
    f_1(t) &= \sin\left[\omega_0(t-\tau)+\omega_0\tau\right]u(t-\tau)\\
    &= \sin\left[\omega_0(t-\tau)\right]\cos(\omega_0\tau)u(t-\tau)\\
    &+ \cos\left[\omega_0(t-\tau)\right]\sin(\omega_0\tau)u(t-\tau)\\
    F_1(s) &= \cos(\omega_0\tau)\frac{\omega_0}{s^2 + \omega_0^2} e^{-s\tau}\\
    &+ \boxed{\sin(\omega_0\tau)\frac{s}{s^2 + \omega_0^2} e^{-s\tau} }
\end{align*}
\section*{4}
\begin{align*}
    g(t) &= f(t) + f(t-T_0) + f(t-2T_0) + \ldots\\
    G(s) &= F(s) + F(s)e^{-sT_0} + F(s)e^{-s2T_0} + \ldots\\
\end{align*}
Let $x = e^{-sT_0}$
\begin{align*}
    G(s) &= F(s)\left(1+x+x^2+x^3+\ldots\right)\\
    &= \frac{F(s)}{1+x}\\
    &= \boxed{\frac{F(s)}{1+e^{-sT_0}}}
\end{align*}
\section*{5}
\begin{align*}
    f(t) &= t\left[ u(t) - u(t-2) \right] + \left( -2t+6 \right)\left[ u(t-2) - u(t-3) \right]\\
    f(0^{-}) &= 0\\
    f'(t)&= u(t)-u(t-2)-2u(t-2)+2u(t-3)\\
    &+6\delta(t-2)-6\delta(t-3)\\
    \mathcal{L}\{ f'(t)\} &= sF(s)-f(0^-)\\
    sF(s) &= \frac{1}{s} - \frac{1}{s} e^{-2s} - \frac{2}{s} e^{-2s} + \frac{2}{s} e^{-3s} +6e^{-2s} -6e^{-3s}\\
    F(s) &= \boxed{\frac{1}{s^2}-\frac{3}{s^2}e^{-2s}+\frac{2}{s^2}e^{-3s} + \frac{6}{s}e^{-2s} - \frac{6}{s}e^{-3s}}
\end{align*}
\end{multicols}
\end{document}
