\documentclass{article}

\usepackage[letterpaper, margin=1.3cm]{geometry}
\usepackage[utf8]{inputenc}
\usepackage{siunitx}
\usepackage{mathtools}
\usepackage{multicol}

\title{ECE 240 Assignment 9}
\author{Michael Kwok}
\begin{document}

\maketitle
\begin{multicols}{2}
\section*{1}
\subsection*{i}
$$F(s) = \frac{s+2}{s(s+1)^2}$$
\begin{align*}
    \frac{s+2}{s(s+1)^2} &= \frac{A}{s}+\frac{B}{s+1} + \frac{C}{(s+1)^2}\\
    s+2 &= A(s+1)^2 + Bs(s+1) + Cs\\
    \text{Let } s &= 0:\\
    A &= 2\\
    \text{Let } s &= -1:\\
    1 &= A(0) -B(0) -C\\
    C &= -1\\
    s+2 &= 2(s+1)^2 + B(s^2 + s) - s\\
    2s + 2 &= 2(s+1)^2 + B(s^2 + s)\\
    2 &= 2(s+1) + Bs\\
    -2s &= Bs\\
    B &= -2\\
    F(s) &= \frac{2}{s} - \frac{2}{s+1} - \frac{1}{(s+1)^2}
\end{align*}
\begin{align*}
\mathcal{L}^{-1}\{F(s)\} &= f(t)\\
&= 2\delta(t) - 2 e^{-t}u(t)-te^{-t}u(t)
\end{align*}
\subsection*{ii}
let $x = e^{-s}$
\begin{align*}
    F(s) = \frac{x+x^2+1}{s^2+3s+2} &= \frac{x+x^2+1}{(s+1)(s+2)}\\
    \frac{x+x^2+1}{(s+1)(s+2)} &= \frac{A}{s+1} + \frac{B}{s+2}\\
    x^2+x+1 &= A(s+2) + B (s+1)\\
    \text{let } s &= -1\\
    A(-1+2) &= e^2 + e + 1\\
    \text{let } s &= -2\\
    B(-2+1) &= e^4 + e^2 + 1\\
    F(s) &= \frac{e^2+e+1}{s+1} - \frac{e^4+e^2+1}{s+2}\\
    f(t) &= e^{-t}u(t)(e^2+e+e)\\
     &- e^{-2}u(t)(e^4+e^2+1)
\end{align*}
\section*{2}
\begin{align*}
&s^2 Y(s) - s y(0^-) - y'(0^-) + 6 sY(s) - 6y(0^-)+25Y(s)\\
&= sF(s) - f(0^-) + 2F(s)\\
\end{align*}
\[
(s^2+6s+25)Y(s) = \overbrace{s+7}^{\text{Zero input}} + \overbrace{sF(s) - f(0^-) + sF(s)}^{\text{Zero state}}
\]
\begin{align*}
    F(s) &= \frac{25}{s}\\
    f(0) &= 0
\end{align*}
\begin{align*}
    Y(s) &= \frac{s+7}{s^2+6s+25} + \frac{25+ \frac{50}{s}}{s^2+6s+25}\\
    &= \frac{(s+3)+4}{(s+3)^2+4^2} + \frac{2}{s} + \frac{13-2s}{s^2+6s+25}\\
    &= \frac{s+3}{(s+3)^2+4^2} + \frac{4}{(s+3)^2+4^2} + \frac{2}{s}\\
    &-2 \frac{s+3}{(s+3)^2+4^2} + \frac{19}{4}\frac{4}{(s+3)^2+4^2}\\
    y(t) &= \overbrace{\left[\left( cos(4t) + sin(4t) \right) e^{-3t} + 2\right]u(t)}^{\text{Zero Input}}\\
    &\overbrace{\left[- 2e^{-3t}cos(4t) + \frac{19}{4}e^{-3t}sin(4t)\right]u(t)}^{\text{Zero State}}
\end{align*}
\section*{3}
\begin{align*}
&s^3 Y(s) + 6s^2 Y(s) -11 sY(s) + 6 Y(s) =\\
&3s^2 F(s) + 7sF(s) +5F(s)
\end{align*}
\begin{align*}
    (s^3 + 6s^2 -11 s + 6) Y(s) &= (3s^2 + 7s +5) F(s)\\
    \frac{Y(s)}{F(s)} &= \boxed{\frac{3s^2 + 7s +5}{s^3 + 6s^2 -11 s + 6}}
\end{align*}
\section*{4}
\subsection*{a}
\begin{align*}
    F(s) &= \frac{1}{s+3}\\
    Y(s) &= \frac{s+5}{(s+2)(s+3)^2}\\
    &= \frac{A}{s+2} + \frac{B}{s+3} + \frac{C}{(s+3)^2}
\end{align*}
    
\begin{align*}
    s+5 = A(s+3)^2 &+ B(s+2)(s+3) + C(s+2)\\
    \text{let } s &= -2,\\
    A &= 3\\
    \text{let } s &= -3,\\
    2 &= C(-3+2)\\
    C &= -2\\
    s+5 &= 3(s+3)^2 + B(s+2)(s+3) + -2(s+2)\\
    -3s^2-15s-18 &= B(s^2+5s+6)\\
    B &+ -3\\
\end{align*}

\begin{align*}
    Y(s) &= \frac{3}{s+2} - \frac{3}{s+3} - \frac{2}{(s+2)^2}\\
    y(t) &= 3 e^{-2t} u(t) - 3 e^{-3t} u(t) - 2t e^{-3t}u(t)\\
    &= \left[ 3e^{-2t} e^{-3t} (3+2t) \right] u(t)
\end{align*}
\subsection*{b}
\begin{align*}
    H(s) &= \frac{s+5}{s^2+5s+6}\\
    (s^2 +5s +6) Y(s) &= (s+5) F(s)\\
    y''(t) + 5 y'(t) + 6y(t) &= f'(t) + 5 f(t)
\end{align*}
\section*{5}
\subsection*{a}
\begin{align*}
    H_1(s) &= \frac{s+1}{s^2+8s+12}\\
    &= \frac{s+1}{(s+2)(s+6)}\\
\end{align*}
Poles at $s_1 = -2, s_2 = -6$

System is BIBO Stable.
\subsection*{b}
$$
H_2(s) = \frac{s+5}{s(s+1)(s+2)}
$$
Poles at $s_1 = 0, s_2 = -1, s_3 = -2$

System is BIBO Unstable.
\subsection*{c}
Poles at $s_1 = 0, s_2 = \sqrt{2}, s_3 = -\sqrt{2}$

System is BIBO Unstable.
\subsection*{d}
Poles at $s_1 = -1, s_2 = 5, s_3 = 1$

System is BIBO Unstable.
\section*{6}
\subsection*{a}
$$\mathcal{L}\{H(s)\} = e^{-2t}u(t)$$
\subsection*{b}
$s = \sigma + j\omega$

Fourier transform is identical to Laplace at $\sigma = 0$, basically a special case of the Laplace transform.

\begin{align*}
    H(j\omega) &= \frac{1}{j\omega + 2}\\
    \mathcal{F}\{H(j\omega)\} &= e^{-2t} u(t)\\
\end{align*}
\end{multicols}
\end{document}
