\documentclass{article}

\usepackage[letterpaper, margin=1.3cm]{geometry}
\usepackage[utf8]{inputenc}
\usepackage{siunitx}
\usepackage{mathtools}
\usepackage{multicol}

\title{ECE 240 Assignment 7}
\author{Michael Kwok}
\begin{document}

\maketitle
\begin{multicols}{2}
\section*{1}

$$f(t) = e^{-1} t \left[ u(t)-u(t-1) \right] + e^{-t}[u(t-1)]$$

\begin{align*}
    F(\omega) &= \int_{-\infty}^{\infty}\left[ e^{-1} t \left[ u(t)-u(t-1) \right] + e^{-t}[u(t-1)]\right]e^{-j\omega t}dt\\
    &= \int_0^1 e^{-1} t e^{-j\omega t} dt + \int_1^\infty e^{-t} e^{-j\omega t} dt\\
    &= e^{-1}\left.\left(\frac{t}{-j\omega} + \frac{1}{\omega^2}\right) e^{-j\omega t}\right\rvert^1_0 + \int_1^\infty e^{-t (1 +j\omega)} dt\\
    &= e^{-1}\left[\left(\frac{1}{-j\omega} + \frac{1}{\omega^2}\right) e^{-j\omega}-\frac{1}{\omega ^2}\right] - \left.\frac{e^{-t (1 +j\omega)}}{1+j\omega} \right\rvert^\infty_0\\
    &= \frac{(j\omega +1) e^{-1-j\omega}-e^{-1}}{\omega ^2} + \frac{e^{-1 -j\omega}}{1+j\omega}\\
    \end{align*}
$$
\boxed{F(\omega) = \frac{(j\omega +1) e^{-1-j\omega}-e^{-1}}{\omega ^2} + \frac{e^{-1 -j\omega}}{1+j\omega}}
$$
\section*{2}
\subsection*{a}
Unit impulse response = $h(t) = \mathcal{F}^{-1}\{H(\omega)\}$
$$
\boxed{h(t) = e^{-2t}u(t)}
$$
\subsection*{b}
$$
Y\{\delta(t)\} = h(t)
$$
\begin{align*}
    Y\{f(t)\} &= y(t)\\
    &= \delta(t)*h(t)
\end{align*}
Using the convolution property of Fourier Transforms,
\begin{align*}
    Y(\omega) &= F(\omega) H(\omega)\\
    &= \left( \frac{1}{2+j\omega} \right) \left( \frac{1}{2+j\omega} \right)
\end{align*}
\begin{align*}
    y(t) &= \int_{-\infty}^{\infty} e^{-2\tau} u(\tau) e^{-2(t-\tau)} u(t-\tau)d\tau\\
    &=\int_0^t e^{-2\tau}e^{2\tau} e^{-2t}d\tau\\
    &= e^{-2t}\int_0^t d\tau\\
    &= \boxed{e^{-2t} t}
\end{align*}
\section*{3}
\begin{align*}
\int_{-\infty}^\infty f_1(t)f_2(t)dt &= \int_{-\infty}^\infty f_1(t)\left[ \int_{-\infty}^\infty F_2(\omega)e^{-j\omega t} d\omega \right]dt\\
&= \frac{1}{2\pi} \int_{-\infty}^\infty F_2(\omega)\left[\int_{-\infty}^\infty f_1(t)e^{-j\omega t}dt\right]d\omega\\
&= \boxed{\frac{1}{2\pi} \int_{-\infty}^\infty F_2(\omega)F_1(-\omega)d\omega}
\end{align*}

OR

\begin{align*}
\int_{-\infty}^\infty f_1(t)f_2(t)dt &= \int_{-\infty}^\infty f_2(t)\left[ \int_{-\infty}^\infty F_1(\omega)e^{-j\omega t} d\omega \right]dt\\
&= \frac{1}{2\pi} \int_{-\infty}^\infty F_1(\omega)\left[\int_{-\infty}^\infty f_2(t)e^{-j\omega t}dt\right]d\omega\\
&= \boxed{\frac{1}{2\pi} \int_{-\infty}^\infty F_1(\omega)F_2(-\omega)d\omega}
\end{align*}
\section*{4}
By duality,
\begin{align*}
    F(\omega) &=2\pi e^{-a|-\omega|}\\
    &= 2\pi e^{-a|\omega|}
\end{align*}
99\% of $E_f$ using $E_f = \int_{-\infty}^\infty|f(t)|^2 dt \rightarrow \frac{1}{2\pi}\int_{-\infty}^\infty |F(\omega)|^2 d\omega$

\begin{align*}
    &\frac{1}{\pi}\int_0^{\omega_B} |F(\omega)|^2 d\omega\\
    =&2\int_0^{\omega_B}e^{-2a\omega}
\end{align*}
\begin{align*}
\int_0^{\omega_B} e^{-2a\omega} &\geq 0.99 \int_0^{\infty} e^{-2a\omega}\\
\frac{2}{a}-\frac{2e^{-2a\omega_B}}{a} &\geq 0.99\cdot\frac{2}{a}\\
1-e^{-2a\omega_B} &\geq 0.99\\
e^{-2a\omega_B} &\leq 0.01\\
2a\omega_B &= 4.6051\\
\omega_B &= \boxed{\frac{2.303}{a}}
\end{align*}

\end{multicols}
\end{document}
=